catering for the multiple contextual patterns in a pattern list (E.g. eq mk_R(x,y) = mk_R(a,b) case now gives an error)

plugins/vdm2isa/java/src/test/resources/TestV2IErrors.thy
@@ -1,8 +1,8 @@
-(* VDM to Isabelle Translation @2021-12-13T14:25:22.241Z
+(* VDM to Isabelle Translation @2022-03-01T08:21:22.905347Z
    Copyright 2021, Leo Freitas, leo.freitas@newcastle.ac.uk
 
-in '/Users/nljsf/Local/reps/git/VDM_Toolkit/plugins/vdm2isa/java/src/test/resources/TestV2IErrors.vdmsl' at line 1:8
-files = [/Users/nljsf/Local/reps/git/VDM_Toolkit/plugins/vdm2isa/java/src/test/resources/TestV2IErrors.vdmsl]
+in './src/test/resources/TestV2IErrors.vdmsl' at line 1:8
+files = [./src/test/resources/TestV2IErrors.vdmsl]
 *)
 theory TestV2IErrors
 imports "VDMToolkit" 
@@ -10,13 +10,15 @@ begin
 
 
 \<comment>\<open>VDM source: S = compose S of  end\<close>
-\<comment>\<open>in 'TestV2IErrors' (/Users/nljsf/Local/reps/git/VDM_Toolkit/plugins/vdm2isa/java/src/test/resources/TestV2IErrors.vdmsl) at line 9:5\<close>
+\<comment>\<open>in 'TestV2IErrors' (./src/test/resources/TestV2IErrors.vdmsl) at line 9:5\<close>
 record S = 
 	
 	
 
-\<comment>\<open>VDM source: inv_S = ?\<close>
-\<comment>\<open>in 'TestV2IErrors' (/Users/nljsf/Local/reps/git/VDM_Toolkit/plugins/vdm2isa/java/src/test/resources/TestV2IErrors.vdmsl) at line 9:5\<close>
+\<comment>\<open>VDM source: inv_S: (S +> bool)
+	inv_S(dummy0) ==
+null\<close>
+\<comment>\<open>in 'TestV2IErrors' (./src/test/resources/TestV2IErrors.vdmsl) at line 9:5\<close>
 definition
 	inv_S :: "S \<Rightarrow> bool"
 where
@@ -25,20 +27,25 @@ where
 		( ( ))"
 
 		
+lemmas inv_S_defs = inv_S_def 
+
 
 	
+	
 \<comment>\<open>VDM source: R = compose R of x:nat, y:nat end
-	inv r == ((r.x) < (r.y))\<close>
-\<comment>\<open>in 'TestV2IErrors' (/Users/nljsf/Local/reps/git/VDM_Toolkit/plugins/vdm2isa/java/src/test/resources/TestV2IErrors.vdmsl) at line 11:5\<close>
+	inv r == ((r.x) < (r.y))
+	eq mk_R(x1, y1) = mk_R(x2, y2) == ((x1 = x2) and (y1 = y2))\<close>
+\<comment>\<open>in 'TestV2IErrors' (./src/test/resources/TestV2IErrors.vdmsl) at line 11:5\<close>
 record R = 
 	x\<^sub>R :: "VDMNat"
+		 
 		 y\<^sub>R :: "VDMNat"
 	
 
 \<comment>\<open>VDM source: inv_R: (R +> bool)
 	inv_R(r) ==
 ((r.x) < (r.y))\<close>
-\<comment>\<open>in 'TestV2IErrors' (/Users/nljsf/Local/reps/git/VDM_Toolkit/plugins/vdm2isa/java/src/test/resources/TestV2IErrors.vdmsl) at line 14:9\<close>
+\<comment>\<open>in 'TestV2IErrors' (./src/test/resources/TestV2IErrors.vdmsl) at line 14:9\<close>
 definition
 	inv_R :: "R \<Rightarrow> bool"
 where
@@ -47,18 +54,41 @@ where
 		( (((inv_VDMNat (x\<^sub>R r))) \<and> 
 		 ((inv_VDMNat (y\<^sub>R r))) ))  \<and> 
 		\<comment>\<open>User defined body of inv_R.\<close>
-		((x\<^sub>R (r)) < (y\<^sub>R (r)))"
+		((x\<^sub>R r) < (y\<^sub>R r))"
 
 		
 
+\<comment>\<open>VDM source: eq_R: (R * R +> bool)
+	eq_R(mk_R(x1, y1), mk_R(x2, y2)) ==
+((x1 = x2) and (y1 = y2))\<close>
+\<comment>\<open>in 'TestV2IErrors' (./src/test/resources/TestV2IErrors.vdmsl) at line 15:8\<close>
+definition
+	eq_R :: "R \<Rightarrow> R \<Rightarrow> bool"
+where
+	"eq_R dummy0   dummy0 \<equiv> 
+		\<comment>\<open>Implicitly defined type invariant checks for  `eq_R` specification.\<close>
+		(inv_R dummy0  \<and>  inv_R dummy0)  \<and> 
+		\<comment>\<open>Implicit pattern context conversion\<close>
+		(let x1 = (x\<^sub>R dummy0); y1 = (y\<^sub>R dummy0); 
+			x1 = (x\<^sub>R dummy0); y1 = (y\<^sub>R dummy0) in 
+		\<comment>\<open>User defined body of eq_R.\<close>
+		((x1 = x2) \<and> (y1 = y2)))"
+
+		
+lemmas inv_R_defs = inv_R_def inv_VDMNat_def 
+
+
+	
 	
 \<comment>\<open>VDM source: TUnion = set of (real)\<close>
-\<comment>\<open>in 'TestV2IErrors' (/Users/nljsf/Local/reps/git/VDM_Toolkit/plugins/vdm2isa/java/src/test/resources/TestV2IErrors.vdmsl) at line 18:5\<close>
+\<comment>\<open>in 'TestV2IErrors' (./src/test/resources/TestV2IErrors.vdmsl) at line 19:5\<close>
 type_synonym TUnion = "U_VDMReal "VDMReal" VDMSet"
 	
 
-\<comment>\<open>VDM source: inv_TUnion = ?\<close>
-\<comment>\<open>in 'TestV2IErrors' (/Users/nljsf/Local/reps/git/VDM_Toolkit/plugins/vdm2isa/java/src/test/resources/TestV2IErrors.vdmsl) at line 18:5\<close>
+\<comment>\<open>VDM source: inv_TUnion: (TUnion +> bool)
+	inv_TUnion(dummy0) ==
+null\<close>
+\<comment>\<open>in 'TestV2IErrors' (./src/test/resources/TestV2IErrors.vdmsl) at line 19:5\<close>
 definition
 	inv_TUnion :: "TUnion \<Rightarrow> bool"
 where
@@ -67,15 +97,20 @@ where
 		(((inv_VDMSet' (inv_TUnion ) dummy0)))"
 
 		 
+lemmas inv_TUnion_defs = inv_TUnion_def inv_VDMReal_def inv_VDMSet'_def inv_VDMSet'_defs 
+
 
 	
+	
 \<comment>\<open>VDM source: TInnerUnion = real\<close>
-\<comment>\<open>in 'TestV2IErrors' (/Users/nljsf/Local/reps/git/VDM_Toolkit/plugins/vdm2isa/java/src/test/resources/TestV2IErrors.vdmsl) at line 21:5\<close>
+\<comment>\<open>in 'TestV2IErrors' (./src/test/resources/TestV2IErrors.vdmsl) at line 22:5\<close>
 datatype TInnerUnion = U_VDMReal "VDMReal"
 	
 
-\<comment>\<open>VDM source: inv_TInnerUnion = ?\<close>
-\<comment>\<open>in 'TestV2IErrors' (/Users/nljsf/Local/reps/git/VDM_Toolkit/plugins/vdm2isa/java/src/test/resources/TestV2IErrors.vdmsl) at line 21:5\<close>
+\<comment>\<open>VDM source: inv_TInnerUnion: (TInnerUnion +> bool)
+	inv_TInnerUnion(dummy0) ==
+null\<close>
+\<comment>\<open>in 'TestV2IErrors' (./src/test/resources/TestV2IErrors.vdmsl) at line 22:5\<close>
 definition
 	inv_TInnerUnion :: "TInnerUnion \<Rightarrow> bool"
 where
@@ -86,28 +121,36 @@ where
 		 )))"
 
 		 
+lemmas inv_TInnerUnion_defs = inv_TInnerUnion_def inv_VDMReal_def 
+
 
 	
+	
 \<comment>\<open>VDM source: TInnerUnion' = set of (TInnerUnion)\<close>
-\<comment>\<open>in 'TestV2IErrors' (/Users/nljsf/Local/reps/git/VDM_Toolkit/plugins/vdm2isa/java/src/test/resources/TestV2IErrors.vdmsl) at line 22:5\<close>
+\<comment>\<open>in 'TestV2IErrors' (./src/test/resources/TestV2IErrors.vdmsl) at line 23:5\<close>
 type_synonym TInnerUnion' = "TInnerUnion VDMSet"
 	
 
-\<comment>\<open>VDM source: inv_TInnerUnion' = ?\<close>
-\<comment>\<open>in 'TestV2IErrors' (/Users/nljsf/Local/reps/git/VDM_Toolkit/plugins/vdm2isa/java/src/test/resources/TestV2IErrors.vdmsl) at line 22:5\<close>
+\<comment>\<open>VDM source: inv_TInnerUnion': (TInnerUnion' +> bool)
+	inv_TInnerUnion'(dummy0) ==
+null\<close>
+\<comment>\<open>in 'TestV2IErrors' (./src/test/resources/TestV2IErrors.vdmsl) at line 23:5\<close>
 definition
 	inv_TInnerUnion' :: "TInnerUnion' \<Rightarrow> bool"
 where
 	"inv_TInnerUnion' dummy0 \<equiv> 
 		\<comment>\<open>Implicitly defined type invariant checks for undeclared `inv_TInnerUnion'` specification.\<close>
-		(((inv_VDMSet' (inv_TInnerUnion) dummy0)))"
+		(((inv_VDMSet' ((inv_TInnerUnion )) dummy0)))"
 
 		 
+lemmas inv_TInnerUnion'_defs = inv_TInnerUnion_def inv_TInnerUnion'_def inv_VDMReal_def inv_VDMSet'_def inv_VDMSet'_defs 
 
+
+	
 	
 \<comment>\<open>VDM source: E = compose E of e:set of (int) end
 	inv mk_E({i, j, k}) == ((i < j) and (j < k))\<close>
-\<comment>\<open>in 'TestV2IErrors' (/Users/nljsf/Local/reps/git/VDM_Toolkit/plugins/vdm2isa/java/src/test/resources/TestV2IErrors.vdmsl) at line 25:5\<close>
+\<comment>\<open>in 'TestV2IErrors' (./src/test/resources/TestV2IErrors.vdmsl) at line 26:5\<close>
 record E = 
 	e\<^sub>E :: "VDMInt VDMSet"
 	
@@ -115,7 +158,7 @@ record E =
 \<comment>\<open>VDM source: inv_E: (E +> bool)
 	inv_E(mk_E({i, j, k})) ==
 ((i < j) and (j < k))\<close>
-\<comment>\<open>in 'TestV2IErrors' (/Users/nljsf/Local/reps/git/VDM_Toolkit/plugins/vdm2isa/java/src/test/resources/TestV2IErrors.vdmsl) at line 26:9\<close>
+\<comment>\<open>in 'TestV2IErrors' (./src/test/resources/TestV2IErrors.vdmsl) at line 27:9\<close>
 definition
 	inv_E :: "E \<Rightarrow> bool"
 where
@@ -128,11 +171,14 @@ where
 		((i < j) \<and> (j < k)))"
 
 		
+lemmas inv_E_defs = inv_E_def inv_VDMInt_def inv_VDMSet'_def inv_VDMSet'_defs 
 
+
+	
 	
 \<comment>\<open>VDM source: F = compose F of f:seq of (int) end
 	inv mk_F(s ^ t) == ((len s) < (len t))\<close>
-\<comment>\<open>in 'TestV2IErrors' (/Users/nljsf/Local/reps/git/VDM_Toolkit/plugins/vdm2isa/java/src/test/resources/TestV2IErrors.vdmsl) at line 29:5\<close>
+\<comment>\<open>in 'TestV2IErrors' (./src/test/resources/TestV2IErrors.vdmsl) at line 30:5\<close>
 record F = 
 	f\<^sub>F :: "VDMInt VDMSeq"
 	
@@ -140,7 +186,7 @@ record F =
 \<comment>\<open>VDM source: inv_F: (F +> bool)
 	inv_F(mk_F(s ^ t)) ==
 ((len s) < (len t))\<close>
-\<comment>\<open>in 'TestV2IErrors' (/Users/nljsf/Local/reps/git/VDM_Toolkit/plugins/vdm2isa/java/src/test/resources/TestV2IErrors.vdmsl) at line 30:9\<close>
+\<comment>\<open>in 'TestV2IErrors' (./src/test/resources/TestV2IErrors.vdmsl) at line 31:9\<close>
 definition
 	inv_F :: "F \<Rightarrow> bool"
 where
@@ -153,45 +199,92 @@ where
 		((len s) < (len t)))"
 
 		
+lemmas inv_F_defs = inv_F_def inv_VDMInt_def inv_VDMSeq'_def inv_VDMSeq'_defs 
 
+
+	
 	
 \<comment>\<open>VDM source: T = set of (nat)
 	inv {a, b, c} == ((a < b) and (b < c))\<close>
-\<comment>\<open>in 'TestV2IErrors' (/Users/nljsf/Local/reps/git/VDM_Toolkit/plugins/vdm2isa/java/src/test/resources/TestV2IErrors.vdmsl) at line 33:5\<close>
+\<comment>\<open>in 'TestV2IErrors' (./src/test/resources/TestV2IErrors.vdmsl) at line 34:5\<close>
 type_synonym T = "VDMNat VDMSet"
 	
 
 \<comment>\<open>VDM source: inv_T: (set of (nat) +> bool)
 	inv_T({a, b, c}) ==
 ((a < b) and (b < c))\<close>
-\<comment>\<open>in 'TestV2IErrors' (/Users/nljsf/Local/reps/git/VDM_Toolkit/plugins/vdm2isa/java/src/test/resources/TestV2IErrors.vdmsl) at line 34:9\<close>
+\<comment>\<open>in 'TestV2IErrors' (./src/test/resources/TestV2IErrors.vdmsl) at line 35:9\<close>
 definition
 	inv_T :: "T \<Rightarrow> bool"
 where
-	"inv_T {a,  b,  c} \<equiv> 
+	"inv_T {a ,  b ,  c} \<equiv> 
 		\<comment>\<open>Implicitly defined type invariant checks for  `inv_T` specification.\<close>
-		(((inv_VDMSet' (inv_VDMNat) {a,  b,  c})))  \<and> 
+		(((inv_VDMSet' (inv_VDMNat) {a ,  b ,  c})))  \<and> 
 		\<comment>\<open>User defined body of inv_T.\<close>
 		((a < b) \<and> (b < c))"
 
 		 
+lemmas inv_T_defs = inv_T_def inv_VDMNat_def inv_VDMSet'_def inv_VDMSet'_defs 
 
+
+	
+	
+\<comment>\<open>VDM source: R2 = compose R2 of x:nat end
+	ord r1 < r2 == ((r1.x) < (r2.x))\<close>
+\<comment>\<open>in 'TestV2IErrors' (./src/test/resources/TestV2IErrors.vdmsl) at line 42:5\<close>
+record R2 = 
+	x\<^sub>R\<^sub>2 :: "VDMNat"
+	
+
+\<comment>\<open>VDM source: inv_R2: (R2 +> bool)
+	inv_R2(dummy0) ==
+null\<close>
+\<comment>\<open>in 'TestV2IErrors' (./src/test/resources/TestV2IErrors.vdmsl) at line 42:5\<close>
+definition
+	inv_R2 :: "R2 \<Rightarrow> bool"
+where
+	"inv_R2 dummy0 \<equiv> 
+		\<comment>\<open>Implicitly defined type invariant checks for undeclared `inv_R2` specification.\<close>
+		( (((inv_VDMNat (x\<^sub>R\<^sub>2 dummy0))) ))"
+ 
+
+\<comment>\<open>VDM source: ord_R2: (R2 * R2 +> bool)
+	ord_R2(r1, r2) ==
+((r1.x) < (r2.x))\<close>
+\<comment>\<open>in 'TestV2IErrors' (./src/test/resources/TestV2IErrors.vdmsl) at line 44:9\<close>
+definition
+	ord_R2 :: "R2 \<Rightarrow> R2 \<Rightarrow> bool"
+where
+	"ord_R2 r1   r2 \<equiv> 
+		\<comment>\<open>Implicitly defined type invariant checks for  `ord_R2` specification.\<close>
+		(inv_R2 r1  \<and>  inv_R2 r2)  \<and> 
+		\<comment>\<open>User defined body of ord_R2.\<close>
+		((x\<^sub>R\<^sub>2 r1) < (x\<^sub>R\<^sub>2 r2))"
+ 
+lemmas inv_R2_defs = inv_R2_def inv_VDMNat_def 
+
+
+	
 	
 \<comment>\<open>VDM source: vc33: (() -> seq of (nat))
 	vc33() ==
 [x | x:nat & (x > 10)]\<close>
-\<comment>\<open>in 'TestV2IErrors' (/Users/nljsf/Local/reps/git/VDM_Toolkit/plugins/vdm2isa/java/src/test/resources/TestV2IErrors.vdmsl) at line 44:5\<close>
+\<comment>\<open>in 'TestV2IErrors' (./src/test/resources/TestV2IErrors.vdmsl) at line 49:5\<close>
 
-\<comment>\<open>VDM source: pre_vc33 = ?\<close>
-\<comment>\<open>in 'TestV2IErrors' (/Users/nljsf/Local/reps/git/VDM_Toolkit/plugins/vdm2isa/java/src/test/resources/TestV2IErrors.vdmsl) at line 44:5\<close>
+\<comment>\<open>VDM source: pre_vc33: (() +> bool)
+	pre_vc33() ==
+null\<close>
+\<comment>\<open>in 'TestV2IErrors' (./src/test/resources/TestV2IErrors.vdmsl) at line 49:5\<close>
 definition
 	pre_vc33 :: "bool"
 where
 	"pre_vc33  \<equiv> True"
 
 
-\<comment>\<open>VDM source: post_vc33 = ?\<close>
-\<comment>\<open>in 'TestV2IErrors' (/Users/nljsf/Local/reps/git/VDM_Toolkit/plugins/vdm2isa/java/src/test/resources/TestV2IErrors.vdmsl) at line 44:5\<close>
+\<comment>\<open>VDM source: post_vc33: (seq of (nat) +> bool)
+	post_vc33(RESULT) ==
+null\<close>
+\<comment>\<open>in 'TestV2IErrors' (./src/test/resources/TestV2IErrors.vdmsl) at line 49:5\<close>
 definition
 	post_vc33 :: "VDMNat VDMSeq \<Rightarrow> bool"
 where
@@ -207,15 +300,18 @@ where
 	[ x . \<comment>\<open>Type bound sequence compression is not supported in Isabelle.\<close>  (((inv_VDMNat x))) , (x > (10::VDMNat1)) ]"
 
 	
+	
 \<comment>\<open>VDM source: f1: (int -> (<ERROR> | bool))
 	f1(x) ==
 (if (x > 10)
 then <ERROR>
 else false)\<close>
-\<comment>\<open>in 'TestV2IErrors' (/Users/nljsf/Local/reps/git/VDM_Toolkit/plugins/vdm2isa/java/src/test/resources/TestV2IErrors.vdmsl) at line 48:5\<close>
+\<comment>\<open>in 'TestV2IErrors' (./src/test/resources/TestV2IErrors.vdmsl) at line 53:5\<close>
 
-\<comment>\<open>VDM source: pre_f1 = ?\<close>
-\<comment>\<open>in 'TestV2IErrors' (/Users/nljsf/Local/reps/git/VDM_Toolkit/plugins/vdm2isa/java/src/test/resources/TestV2IErrors.vdmsl) at line 48:5\<close>
+\<comment>\<open>VDM source: pre_f1: (int +> bool)
+	pre_f1(x) ==
+null\<close>
+\<comment>\<open>in 'TestV2IErrors' (./src/test/resources/TestV2IErrors.vdmsl) at line 53:5\<close>
 definition
 	pre_f1 :: "VDMInt \<Rightarrow> bool"
 where
@@ -224,13 +320,15 @@ where
 		((inv_VDMInt x))"
 
 
-\<comment>\<open>VDM source: post_f1 = ?\<close>
-\<comment>\<open>in 'TestV2IErrors' (/Users/nljsf/Local/reps/git/VDM_Toolkit/plugins/vdm2isa/java/src/test/resources/TestV2IErrors.vdmsl) at line 48:5\<close>
+\<comment>\<open>VDM source: post_f1: (int * (<ERROR> | bool) +> bool)
+	post_f1(x, RESULT) ==
+null\<close>
+\<comment>\<open>in 'TestV2IErrors' (./src/test/resources/TestV2IErrors.vdmsl) at line 53:5\<close>
 definition
-	post_f1 :: "VDMInt\<Rightarrow> U_ERROR  | 
+	post_f1 :: "VDMInt \<Rightarrow> U_ERROR  | 
 		 U_bool "bool" \<Rightarrow> bool"
 where
-	"post_f1 x  RESULT \<equiv> 
+	"post_f1 x   RESULT \<equiv> 
 		\<comment>\<open>Implicitly defined type invariant checks for undeclared `post_f1` specification.\<close>
 		((inv_VDMInt x)  \<and>  (case RESULT of U_ERROR  \<Rightarrow> (inv_True RESULT)
 		  | U_bool RESULT \<Rightarrow> (inv_bool RESULT)
@@ -249,13 +347,16 @@ where
 		((False::\<bool>)))"
 
 	
+	
 \<comment>\<open>VDM source: f1': (int -> <ERROR>)
 	f1'(-) ==
 <ERROR>\<close>
-\<comment>\<open>in 'TestV2IErrors' (/Users/nljsf/Local/reps/git/VDM_Toolkit/plugins/vdm2isa/java/src/test/resources/TestV2IErrors.vdmsl) at line 52:5\<close>
+\<comment>\<open>in 'TestV2IErrors' (./src/test/resources/TestV2IErrors.vdmsl) at line 57:5\<close>
 
-\<comment>\<open>VDM source: pre_f1' = ?\<close>
-\<comment>\<open>in 'TestV2IErrors' (/Users/nljsf/Local/reps/git/VDM_Toolkit/plugins/vdm2isa/java/src/test/resources/TestV2IErrors.vdmsl) at line 52:5\<close>
+\<comment>\<open>VDM source: pre_f1': (int +> bool)
+	pre_f1'(-) ==
+null\<close>
+\<comment>\<open>in 'TestV2IErrors' (./src/test/resources/TestV2IErrors.vdmsl) at line 57:5\<close>
 definition
 	pre_f1' :: "VDMInt \<Rightarrow> bool"
 where
@@ -264,12 +365,14 @@ where
 		((inv_VDMInt dummy0_ignore))"
 
 
-\<comment>\<open>VDM source: post_f1' = ?\<close>
-\<comment>\<open>in 'TestV2IErrors' (/Users/nljsf/Local/reps/git/VDM_Toolkit/plugins/vdm2isa/java/src/test/resources/TestV2IErrors.vdmsl) at line 52:5\<close>
+\<comment>\<open>VDM source: post_f1': (int * <ERROR> +> bool)
+	post_f1'(-, RESULT) ==
+null\<close>
+\<comment>\<open>in 'TestV2IErrors' (./src/test/resources/TestV2IErrors.vdmsl) at line 57:5\<close>
 definition
-	post_f1' :: "VDMInt\<Rightarrow> U_ERROR  \<Rightarrow> bool"
+	post_f1' :: "VDMInt \<Rightarrow> U_ERROR  \<Rightarrow> bool"
 where
-	"post_f1' dummy0_ignore  RESULT \<equiv> 
+	"post_f1' dummy0_ignore   RESULT \<equiv> 
 		\<comment>\<open>Implicitly defined type invariant checks for undeclared `post_f1'` specification.\<close>
 		((inv_VDMInt dummy0_ignore)  \<and>  (inv_True RESULT))"
 
@@ -281,8 +384,46 @@ where
 	U_ERROR "
 
 	
+	
+\<comment>\<open>VDM source: rcomp: (R2 * R2 -> bool)
+	rcomp(r0, r1) ==
+(r0 >= r1)\<close>
+\<comment>\<open>in 'TestV2IErrors' (./src/test/resources/TestV2IErrors.vdmsl) at line 61:5\<close>
+
+\<comment>\<open>VDM source: pre_rcomp: (R2 * R2 +> bool)
+	pre_rcomp(r0, r1) ==
+null\<close>
+\<comment>\<open>in 'TestV2IErrors' (./src/test/resources/TestV2IErrors.vdmsl) at line 61:5\<close>
+definition
+	pre_rcomp :: "R2 \<Rightarrow> R2 \<Rightarrow> bool"
+where
+	"pre_rcomp r0   r1 \<equiv> 
+		\<comment>\<open>Implicitly defined type invariant checks for undeclared `pre_rcomp` specification.\<close>
+		(inv_R2 r0  \<and>  inv_R2 r1)"
+
+
+\<comment>\<open>VDM source: post_rcomp: (R2 * R2 * bool +> bool)
+	post_rcomp(r0, r1, RESULT) ==
+null\<close>
+\<comment>\<open>in 'TestV2IErrors' (./src/test/resources/TestV2IErrors.vdmsl) at line 61:5\<close>
+definition
+	post_rcomp :: "R2 \<Rightarrow> R2 \<Rightarrow> bool \<Rightarrow> bool"
+where
+	"post_rcomp r0   r1   RESULT \<equiv> 
+		\<comment>\<open>Implicitly defined type invariant checks for undeclared `post_rcomp` specification.\<close>
+		(inv_R2 r0  \<and>  inv_R2 r1  \<and>  (inv_bool RESULT))"
+
+definition
+	rcomp :: "R2 \<Rightarrow> R2 \<Rightarrow> bool"
+where
+	"rcomp r0   r1 \<equiv> 
+	\<comment>\<open>User defined body of rcomp.\<close>
+	(r0 \<ge> r1)"
+
+	
+	
 \<comment>\<open>VDM source: v65:R = mk_R(1, 2)\<close>
-\<comment>\<open>in 'TestV2IErrors' (/Users/nljsf/Local/reps/git/VDM_Toolkit/plugins/vdm2isa/java/src/test/resources/TestV2IErrors.vdmsl) at line 56:5\<close>
+\<comment>\<open>in 'TestV2IErrors' (./src/test/resources/TestV2IErrors.vdmsl) at line 65:5\<close>
 abbreviation
 	v65 :: "R"
 where
@@ -291,12 +432,13 @@ where
 	definition
 	inv_v65 :: "\<bool>"
 where
-	"inv_v65  \<equiv> inv_R v65"
+	"inv_v65  \<equiv> inv_R  v65"
 
 	
 	
+	
 \<comment>\<open>VDM source: v830:seq of (nat) = [x | mk_R(x, -) in set {v65} & (0 < x)]\<close>
-\<comment>\<open>in 'TestV2IErrors' (/Users/nljsf/Local/reps/git/VDM_Toolkit/plugins/vdm2isa/java/src/test/resources/TestV2IErrors.vdmsl) at line 61:5\<close>
+\<comment>\<open>in 'TestV2IErrors' (./src/test/resources/TestV2IErrors.vdmsl) at line 70:5\<close>
 abbreviation
 	v830 :: "VDMNat VDMSeq"
 where
@@ -310,33 +452,34 @@ where
 
 	
 	
+	
 \<comment>\<open>VDM source: v954:map (nat1) to (nat1) = {(x + y) |-> 10 | [x, y] in set {[1, 2], [3, 4], [4, 5]}}\<close>
-\<comment>\<open>in 'TestV2IErrors' (/Users/nljsf/Local/reps/git/VDM_Toolkit/plugins/vdm2isa/java/src/test/resources/TestV2IErrors.vdmsl) at line 65:5\<close>
+\<comment>\<open>in 'TestV2IErrors' (./src/test/resources/TestV2IErrors.vdmsl) at line 74:5\<close>
 abbreviation
 	v954 :: "(VDMNat1 \<rightharpoonup> VDMNat1)"
 where
 	"v954 \<equiv> (\<comment>\<open>VDM Map comprehension is translated as a lambda-term through mapCompSetBound\<close>
 		mapCompSetBound 
-		{(x+y)} 
+		{(x + y)} 
 		{(10::VDMNat1)} 
 		(inv_VDMNat1) 
 		(inv_VDMNat1) 
 		(
-	\<lambda> (dummy0DOMAIN :: VDMNat1)  (dummy0RANGE :: VDMNat1) .
-		(if (((inv_VDMNat1 dummy0DOMAIN))) \<and>  (((inv_VDMNat1 dummy0RANGE))) \<and> (inv_VDMNat1 (
-		if ((\<exists> (dummy0DOMAIN :: VDMNat1)  (dummy0DOMAIN :: VDMNat1)  . ((((inv_VDMNat1 dummy0DOMAIN))) \<and>  (((inv_VDMNat1 dummy0DOMAIN))) \<longrightarrow> ((dummy0DOMAIN = (x+y)) \<and> (True::\<bool>))))) then
+	\<lambda> (dummy0DOMAIN :: VDMNat1)   (dummy0RANGE :: VDMNat1) .
+		(if (((inv_VDMNat1 dummy0DOMAIN)))  \<and>  (((inv_VDMNat1 dummy0RANGE))) \<and> (inv_VDMNat1 (
+		if ((\<exists> (dummy0DOMAIN :: VDMNat1)   (dummy0DOMAIN :: VDMNat1)  . ((((inv_VDMNat1 dummy0DOMAIN)))  \<and>  (((inv_VDMNat1 dummy0DOMAIN))) \<longrightarrow> ((dummy0DOMAIN = (x + y)) \<and> (True::\<bool>))))) then
 		(dummy0DOMAIN)
 		else
 		(undefined))) then
-		(
-		if ((\<exists> (dummy0DOMAIN :: VDMNat1)  (dummy0DOMAIN :: VDMNat1)  . ((((inv_VDMNat1 dummy0DOMAIN))) \<and>  (((inv_VDMNat1 dummy0DOMAIN))) \<longrightarrow> ((dummy0DOMAIN = (x+y)) \<and> (True::\<bool>))))) then
+			(
+		if ((\<exists> (dummy0DOMAIN :: VDMNat1)   (dummy0DOMAIN :: VDMNat1)  . ((((inv_VDMNat1 dummy0DOMAIN)))  \<and>  (((inv_VDMNat1 dummy0DOMAIN))) \<longrightarrow> ((dummy0DOMAIN = (x + y)) \<and> (True::\<bool>))))) then
 		(dummy0DOMAIN)
 		else
 		(undefined))
-	 else
-		undefined
-	)
-	) 
+		 else
+			undefined
+		)
+		) 
 		(rngcnst (10::VDMNat1)) 
 		(truecnst ))"
 
@@ -347,8 +490,9 @@ where
 
 	
 	
+	
 \<comment>\<open>VDM source: -:nat = 10\<close>
-\<comment>\<open>in 'TestV2IErrors' (/Users/nljsf/Local/reps/git/VDM_Toolkit/plugins/vdm2isa/java/src/test/resources/TestV2IErrors.vdmsl) at line 68:5\<close>
+\<comment>\<open>in 'TestV2IErrors' (./src/test/resources/TestV2IErrors.vdmsl) at line 77:5\<close>
 abbreviation
 	dummy0_ignore :: "VDMNat"
 where
